Beginning to attack last trickiest theorem

doc/formalization/Catala.Translation.fst
@@ -47,17 +47,6 @@ let typ_process_exceptions_f (tau: L.ty)
   assert_norm(L.typing L.empty (process_exceptions_f tau)
       (L.TArrow (L.TOption tau) (L.TArrow (L.TArrow L.TUnit tau) (L.TOption tau))))
 
-noeq type env' = {
-  tys: D.env;
-  max_free: nat
-}
-let env = g:env'{forall (i:nat{i > g.max_free}). g.tys i = None}
-
-let extend (g: env) (x: D.var) (ty: D.ty) : env =
-  let new_tys = D.extend g.tys x ty in
-  let new_max_free = if x > g.max_free then x else g.max_free in
-  { tys = new_tys; max_free = new_max_free }
-
 (**** Main translation *)
 
 let rec translate_exp (e: D.exp) : Tot L.exp = match e with
@@ -103,6 +92,11 @@ let extend_translate_commute (g: D.env) (x: D.var) (tau: D.ty)
   FunctionalExtensionality.extensionality L.var_name (fun _ -> option L.ty)
     (L.extend (translate_env g) x (translate_ty tau))
     (translate_env (D.extend g x tau))
+
+let translate_empty_is_empty () : Lemma (translate_env D.empty == L.empty) =
+  FunctionalExtensionality.extensionality L.var_name (fun _ -> option L.ty)
+    (translate_env D.empty)
+    L.empty
 
 (**** Typing preservation theorem *)
 
@@ -183,3 +177,116 @@ and translation_preserves_typ_exceptions
     assert(L.typing g' hd' tau');
     assert(L.typing g' (L.EAbs L.Silent L.TUnit hd') thunked_tau')
 #pop-options
+
+(*** Translation correctness *)
+
+(**** Helpers *)
+
+let rec l_step_rec (e: L.exp) (fuel: nat) : Tot (option L.exp) (decreases fuel) =
+  match L.step e with
+  | None -> None
+  | Some e' -> if fuel = 0 then Some e' else l_step_rec e' (fuel - 1)
+
+let multiple_l_steps (e1: L.exp) (e2: L.exp) (n: nat) =  l_step_rec e1 n = Some e2
+
+let not_l_value = e:L.exp{not (L.is_value e)}
+
+let step_lift_commute_non_value (f:(L.exp -> not_l_value)) (e: L.exp) =
+  match L.step e, L.is_value e with
+  | None, false -> L.step (f e) = None
+  | Some e', false -> if L.is_value e' then true else L.step (f e) = Some (f e')
+  | _ -> true
+
+let is_stepping_agnostic_lift (f:(L.exp -> not_l_value)) = forall (e: L.exp).
+  step_lift_commute_non_value f e
+
+let stepping_agnostic_lift = f:(L.exp -> not_l_value){is_stepping_agnostic_lift f}
+
+let if_lift (e2 e3: L.exp) : stepping_agnostic_lift =
+  let f : L.exp -> not_l_value = fun (e1: L.exp) -> L.EIf e1 e2 e3 in
+  let aux (e1: L.exp) : Lemma (step_lift_commute_non_value f e1) =
+    match L.step e1 with
+    | None -> ()
+    | Some e' -> ()
+  in
+  Classical.forall_intro aux;
+  f
+
+#push-options "--z3rlimit 50 --fuel 1 --ifuel 1"
+let rec lift_multiple_l_steps
+  (e1: L.exp)
+  (e2: L.exp)
+  (n: nat)
+  (f : stepping_agnostic_lift)
+    : Lemma
+      (requires (multiple_l_steps e1 e2 n))
+      (ensures (multiple_l_steps (f e1) (f e2) n))
+      (decreases n)
+  =
+  match L.step e1 with
+  | None -> ()
+  | Some e1' ->
+    if L.is_value e1' then begin
+      admit()
+    end else if n = 0 then
+      assert(L.step (f e1) = Some (f e2))
+    else lift_multiple_l_steps e1' e2 (n-1) f
+#pop-options
+(**** Main theorems *)
+
+let translation_correctness_value (e: D.exp) : Lemma
+    ((D.is_value e) <==> (L.is_value (translate_exp e)))
+  = ()
+
+#push-options "--fuel 2 --ifuel 1 --z3rlimit 50"
+let rec translation_correctness_step (e: D.exp) : Pure nat
+    (requires (Some? (D.step e)))
+    (ensures (fun n -> multiple_l_steps (translate_exp e) (translate_exp (Some?.v (D.step e))) n))
+  =
+  let e' = translate_exp e in
+  let stepped_e = Some?.v (D.step e) in
+  let stepped_e' = translate_exp stepped_e in
+  match e with
+  | D.EVar _ -> 0
+  | D.ELit _ -> 0
+  | D.EAbs _ _ _ -> 0
+  | D.EIf e1 e2 e3 ->
+     if not (D.is_value e1) then begin
+       let e1' = translate_exp e1 in
+       let e2' = translate_exp e2 in
+       let e3' = translate_exp e3 in
+       let stepped_e1 = Some?.v (D.step e1) in
+       let stepped_e1' = translate_exp stepped_e1 in
+       let n_e1 = translation_correctness_step e1 in
+       lift_multiple_l_steps e1' stepped_e1' n_e1 (fun e1' -> L.EIf e1' e2' e3');
+       n_e1
+     end else admit()
+  | _ -> admit()
+
+(*** Wrap-up theorem  *)
+
+let translation_correctness (e: D.exp) (tau: D.ty)
+    : Lemma
+      (requires (D.typing D.empty e tau))
+      (ensures (
+        let e' = translate_exp e in
+        let tau' = translate_ty tau in
+        L.typing L.empty e' tau' /\ begin
+          if D.is_value e then L.is_value e' else begin
+            D.progress e tau;
+            let stepped_e = Some?.v (D.step e) in
+            let stepped_e' = translate_exp stepped_e in
+            exists (n:nat). multiple_l_steps e' stepped_e' n
+          end
+        end
+      ))
+ =
+ let e' = translate_exp e in
+ let tau' = translate_ty tau in
+ translation_preserves_typ D.empty e tau;
+ translate_empty_is_empty ();
+ if D.is_value e then translation_correctness_value e else begin
+    D.progress e tau;
+    let n = translation_correctness_step e in
+    ()
+ end
